---
title: 微分流形与微分几何 12-Oct-2023
date: 2023-10-12 17:40:00
category: 
- 学科笔记
- 博一(秋)
- 微分几何
tags: 
- 笔记
mathjax: true
---

**Definition** (Differential forms) Consider $M^n$. We say $\omega$ is a $k$-form on $M$ w.r.t. $X^1,\ldots,X^n$, if 
$$
\omega=\sum_{1\leq i_1< \cdots < i_k\leq n}\omega_{i_1\cdots i_k}\operatorname dx^{i_1}\wedge \cdots \operatorname dx^{i_k}.
$$
We define the action 
$$
\omega(X^{j_1},\ldots, X^{j_k})=\sum_{1\leq i_1< \cdots< i_k\leq n}\omega_{i_1\cdots i_k}\det(\operatorname dx^{i_s}(X^{j_t}))_{s,t=1}^n.
$$
**Proposition** $\omega$ is independent of the choice of coordinates. 

> **Proof** In fact, we consider the following coordinate-free definition of differential forms. For $0$-forms, consider $\omega=f \in C^\infty(M)$​. Then
> $$
> \operatorname df:\mathscr X(M)\to C^\infty(M),\quad X\mapsto \operatorname df(X)=Xf.
> $$
> For $1$-forms $\omega \in A^1(M)$, consider 
> $$
> \operatorname d\omega :\mathscr X(M)\times \mathscr X(M)\to C^\infty(M).
> $$
> We write $\omega =\omega_i\operatorname dx^i$, $X=c_k\partial _k$, and $Y=d_k\partial _k$, and find that
> $$
> \begin{align*}
> \operatorname d\omega (X,Y)&=(\partial_i\omega_j)(\operatorname dx^i\wedge\operatorname dx^j)(c_k\partial_k,d_l\partial_l)\\[6pt]
> &=(\partial_i\omega_j)(c_id_j)-(\partial_i\omega_j)(c_jd_i)\\[6pt]
> &=c_i\partial_i(\omega_jd_j)-c_i(\partial_id_j)\omega_j-d_i(\partial_i\omega_j c_j)+d_i(\partial_ic_j)\omega_j\\[6pt]
> &=c_i\partial_i(\omega_jd_j)-d_i(\partial_i\omega_j c_j)-c_i(\partial_id_j)\omega_j+d_i(\partial_ic_j)\omega_j\\[6pt]
> &=X(\omega (Y))-Y(\omega(X))-\omega([X,Y]).
> \end{align*}
> $$
> Then we shall prove that
> $$
> (\operatorname d\omega)(X_1,\ldots,X_{k+1})=(-1)^{i-1}X_i(\omega(\widehat{X_i}))+[(-1)^{i+j}\omega([X_i,X_j],\widehat{X_i},\widehat{X_j})]_{i< j}.
> $$
> Denote the right hand side by $\widetilde{\operatorname d\omega}$. We see that 
>
> * $\widetilde{\operatorname d\omega}$ is anti-symmetric, which is clear by direct verification;
>
> * $\widetilde{\operatorname d\omega}$ is multilinear, equivalently (with previous property),
>   $$
>   \widetilde{\operatorname d\omega}(fX_1,X_2,\ldots,X_n)=f\cdot \widetilde{\operatorname d\omega}(X_1,\ldots, X_n);
>   $$
>
> * $\widetilde{\operatorname d\omega}$ coincides $\operatorname d\omega$ locally, we may take $X_i=\partial_i$ and $\omega =f\operatorname dx^1\wedge\cdots \wedge \operatorname dx^k$, and find 
>   $$
>   \begin{align*}
>   \widetilde{\operatorname d\omega}(\partial_{i_1},\ldots,\partial_{i_{k+1}})&=(-1)^{i-1}\partial_{j_i}(\omega(\widehat{\partial_{j_i}})).
>   \end{align*}
>   $$
>   If $i_1< i_2< \cdots< i_{k+1}$, then the above formula does not vanish unless $i_j=j$ ($1\leq j\leq k$). Then 
>   $$
>   \widetilde{\operatorname d\omega}(\partial_{i_1},\ldots,\partial_{i_{k+1}})=(-1)^{i_{k+1}-1}\partial_{i_{k+1}}(f)=\operatorname d\omega (\partial_{i_1},\ldots,\partial_{i_{k+1}}).
>   $$

**Proposition** Consider $\varphi:M\to N$ the differential map, $\omega\in A^k(N)$. Let $X_1,\ldots, X_k$ be $k$ vector fields on $M$. Then
$$
(\varphi^\ast \omega)(X_1,\ldots,X_k)=\omega(\varphi_\ast X_1,\ldots,\varphi_\ast X_k).
$$

> **Proof** It is clear that
> $$
> (\varphi^\ast \omega)_p(X_1,\ldots,X_k)=\omega_{\varphi(p)}(\varphi_\ast X_1,\ldots,\varphi_\ast X_k).
> $$

**Definition** (Contraction operator) Take $X\in \mathscr X(M)$ and define
$$
i_X:A^k(M)\to A^{k-1}(M),\quad \omega (-) \mapsto \omega(X,-).
$$




























