---
title: 答疑 01-Jun-2023
date: 2023-09-12 11:40:00
category: 
- 答疑
- 2023
- June
tags: 
- 答疑
mathjax: true
---

Q: 证明：$\frac{ {\binom n0} }{m+1}-\frac{ {\binom n1} }{m+2}+\frac{ {\binom n2} }{m+3}-\cdots +(-1)^n\frac{ {\binom n n} }{m+n+1}=\frac{1}{(m+n+1){\binom{m+n} n} }$. 

***

A: 二项式展开表明
$$
(1-x)^n=\sum_{k=0}^n\binom{n}{k}(-x)^k.
$$
因此
$$
(1-x)^n\cdot x^m=\sum_{k=0}^n\binom{n}{k}(-1)^kx^{m+k}.
$$
两侧对 $x\in[0,1]$ 积分, 得
$$
\int_0^1(1-x)^nx^m\mathrm dx=\sum_{k=0}^n\dfrac{\binom{n}{k}\cdot (-1)^k}{m+1+k}.
$$
左式就是著名的 $\beta$-积分了, 
$$
\begin{align*}
\int_0^1(1-x)^mx^n\,\mathrm{d}x
&=\frac{m}{n+1}\frac{m-1}{n+2}\cdots\frac1{n+m}\int_0^1x^{n+m}\,\mathrm{d}x\\[6pt]
&=\frac{m}{n+1}\frac{m-1}{n+2}\cdots\frac1{n+m}\frac1{n+m+1}\\[6pt]
&=\frac{n!\,m!}{(n+m+1)!}\\[6pt]
&=\frac{\Gamma(n+1)\Gamma(m+1)}{\Gamma(n+m+2)}\\[6pt]
&=\mathrm{B}(n+1,m+1).
\end{align*}
$$

***