---
title: 微分流形与微分几何 24-Sept-2023
date: 2023-09-24 17:40:00
category: 
- 学科笔记
- 博一(秋)
- 微分几何
tags: 
- 笔记
mathjax: true
---

## Lie brackets

**Definition** (Lie bracket) $\mathscr X(M)$ consists of vector fields over $M$. Lie bracket is defined as
$$
[,]:\mathscr X(M)\times \mathscr X(M)\to \mathscr X(M),\quad (X,Y)\mapsto [X,Y],
$$
satisfying the following:
1. $[X,Y]+[Y,X]=0$;
2. $[fX,gY]=f(Xg)Y+g(Yf)X$;
3. $[[X,Y],Z]+[[Y,Z],X]+[[Z,X],Y]=0$.

**Definition** (one parametre subgroup generated by vector field over $X$) Given $\gamma:(a,b)\to M$ an orbit (trajectory) of $X\in\mathscr X(M)$, if 
$$
\gamma'(t)=X(\gamma(t))\quad \forall t\in (a,b).
$$

**Lemma** (the theorem of existence and uniqueness of the ODE solution on manifolds) $\forall p\in M$, $p\in \overline V\subseteq U\subseteq M$, there exists $\varepsilon > 0$ and differential map 
$$
\gamma:(-\varepsilon, \varepsilon)\times V\to U,
$$
such that
1. $\forall  q\in V$, we have the initial $\gamma(0,q)=q$;
2. $\forall t\in (-\varepsilon,\varepsilon)$ and $\forall q\in V$, we have that 
$$
\gamma'(t,q)=X(\gamma(t,q)). 
$$
> Here we denote that $\gamma_t(q):=\gamma(t,q)$. 

**Theorem** One parameter subgroup is locally a group. For arbitrary $t_1,t_2\in (-\varepsilon,\varepsilon)$ such that $t_1+t_2\in (-\varepsilon,\varepsilon)$, we have that 
$$
\gamma_{t_1}(\gamma_{t_2}(q))=\gamma_{t_2}(\gamma_{t_2}(q))=\gamma_{t_1+t_2}(q)\quad (\forall q\in V). 
$$
If $t\in \mathbb R$, then $\{\gamma_t\}_{t\in \mathbb R}$ is a group with identity $\gamma_0$ and $\gamma_{-t}=\gamma_t^{-1}$. 

## Lie derivative

**Definition** (Lie derivative) Take $X,Y\in \mathscr X(M)$ non-vanishing on $M$. Define $L_XY$ the Lie derivative of $Y$ w.r.t. $X$ at $p\in M$. Let $\gamma_t$ be one parametre subgroup generated by $X$, then
$$
(L_XY)(p)=\lim_{t\to 0}\dfrac{(\gamma_{-t})_\ast(Y(\gamma_t(p)))-Y(p)}{t}. 
$$

**Theorem** $L_XY=[X,Y]$. 
> **Proof** $\forall f\in C^\infty(M)$, we prove that $(L_XY)(f)=[X,Y](f)$.
> $$
> \begin{align*}
> (L_XY)_p(f)&=\lim_{t\to 0}\dfrac{(\gamma_{-t})_\ast(Y(\gamma_t(p)))-Y(p)}{t}f\\[6pt]
> &=\lim_{t\to 0}\dfrac{Y(\gamma_t(p)) (f\circ \gamma_{-t})-Y(p) f}{t}\\[6pt]
> &=(Y(\gamma_t(p))(f\circ \gamma_{-t}))'_{t=0}\\[6pt]
> &=\left(\dfrac{\partial}{\partial s}(f\circ \gamma_{-t})(\sigma_s(\gamma_t(p)))|_{s=0}\right)'_{t=0}\\[6pt]
> &=\dfrac{\partial^2}{\partial s\partial t}(f\circ \gamma_{-t})(\sigma_s(\gamma_t(p)))|_{s,t=0}\\[6pt]
> &=\dfrac{\partial^2}{\partial s\partial t}(f\circ\sigma_s(\gamma_t(p)))|_{s,t=0}+\dfrac{\partial^2}{\partial s\partial t}(f\circ \gamma_{-t}(\sigma_s(p)))|_{s,t=0}\\[6pt]
> &=\dfrac{\partial}{\partial s}X(f\circ\sigma_s)|_{s=0}+\dfrac{\partial}{\partial t}Y(f\circ \gamma_{-t})|_{t=0}\\[6pt]
> &=X(Yf)-Y(Xf)=[X,Y]f. 
> \end{align*}
> $$