---
title: 微分流形与微分几何 14-Sept-2023
date: 2023-09-14 17:40:00
category: 
- 学科笔记
- 博一(秋)
- 微分几何
tags: 
- 笔记
mathjax: true
---

## Tangent space

**Definition** (tangent space at a point) Let $M$ be a differentiable manifold. The tangent space at $p\in M$ consists of the operator of the form $\dfrac{\partial }{\partial v}|_p$ with $v=r^\prime(0)$ for some curve $\gamma(t)$ starting with $\gamma(0)=p$. 
> In other words, for arbitrary differentiable function on $M$, we have that
> $$
> \dfrac{\partial f}{\partial v}|_p=\dfrac{\mathrm d}{\mathrm dt} f\circ \gamma(t)|_{t=0}=(f\circ \gamma)^\prime(0). 
> $$

**Definition** (tangent curves defined via dual space) We say two differentiable curves
$$
\gamma_i:(-\varepsilon_i,+\varepsilon_i)\to M,0\mapsto p\quad (i\in \{1,2\})
$$
are tangent to each other, whenever the following are satisfied
1. $\gamma_1^\prime(0)=\gamma_2^\prime(0)=v$.
2. For arbitrary differentiable $f:M\to \mathbb R$, we always have $(f\circ \gamma_1)^\prime(0)=(f\circ \gamma_2)^\prime(0)$. 
> It yields an equivalence relation $\sim_{\text{tangent}}$. 

**Definition** (tangent space defined via shoots) Set the set of differentiable curves
$$
\mathscr D_p:=\{\gamma:(-\varepsilon,\varepsilon)\to M\text{ differentiable at }\gamma(0)=p.\},
$$
we define the tangent space as $T_pM:=\mathscr D_p/\sim_{\text{tagent}}$ for arbitrary $p\in M$. 

**Proposition** ($T_pM$ is $\mathbb R$-linear) Take $(U,\varphi)$ the chart of $M$ with $p\in U$. WLOG define the coordinate system $(x^1,\ldots, x^n)$ with $\varphi(p)=(0,\ldots,0)$. 
1. To verify that $[\gamma_1]+[\gamma_2]=[\varphi^{-1}(\varphi\circ \gamma_1+\varphi\circ \gamma_2)]$, we need to prove that the right hand side is independent w.r.t. $\varphi$ and $[\gamma_i]$'s. In other words, the following is supposed to hold
$$
\begin{align*}
&(f\circ (\varphi^{-1}(\varphi\circ \gamma_1+\varphi\circ \gamma_2)))^\prime (0)\\[6pt]
\overset {\text{(a)}}=\,&(f\circ (\varphi^{-1}(\varphi\circ \overline{\gamma_1}+\varphi\circ \overline{\gamma_2})))^\prime (0)\\[6pt]
\overset {\text{(b)}}=\,&(f\circ (\overline \varphi^{-1}(\overline\varphi\circ \overline{\gamma_1}+\overline\varphi\circ \overline{\gamma_2})))^\prime (0).
\end{align*}
$$
Here $(\text a)$ is trivial as we derivate $(f\circ \varphi^{-1})\circ (\varphi\circ \gamma_1+\varphi\circ \gamma_2)$. $(\text b)$ is due to $f\circ \overline \varphi^{-1}=f\circ \varphi^{-1}\circ \varphi\circ \overline \varphi^{-1}$
2. To verify that $\lambda[\gamma]=[\varphi^{-1}(\varphi(\lambda \gamma))]$, repeat 1. 

**Proposition** ($\mathbb R$-basis of $T_pM$) Now we consider $\dim M=n$ and 
$$
\gamma_i(t):=\varphi^{-1}((0,\ldots, 0,\underset{\substack{\uparrow\\\boxed{i^\text{th}}}}t,0,\ldots, 0))\quad 1\leq i\leq n.
$$
1. $[\gamma]\in T_pM$, we consider 
$$
(\varphi\circ \gamma)(t)=(x^1(t),\ldots,x^n(t)),\quad \alpha_i:=\dfrac{\mathrm dx^i}{\mathrm dt}|_{t=0}.
$$
Then $[\gamma]=[\varphi^{-1}(x^1(t),\ldots ,x^n(t))]=[\varphi^{-1}(\alpha_1t,\ldots ,\alpha^nt)]=\sum_{1\leq i\leq n}\alpha_i[\gamma_i]$. 
2. The linear independence is clear. 

**Proposition** In fact, $[\gamma_i]=\dfrac{\partial }{\partial x^i}|_p$, since for arbitrary $f\in C^\infty(M)$,
$$
\begin{align*}
&(f\circ \gamma_i)'(0)=((f\circ \varphi^{-1})\circ (\varphi\circ \gamma_i))'(0)\\[6pt]
=\,&((\dfrac{\partial (f\circ \varphi^{-1})}{\partial x^1},\ldots, \dfrac{\partial (f\circ \varphi^{-n})}{\partial x^n})\circ (0,\ldots,0,1,0,\ldots,0)^T)'(0)\\[6pt]
=\,&\dfrac{\partial (f\circ \varphi^{-1})}{\partial x^i}_{\varphi (p)}=\dfrac{\partial f}{\partial x^i}|_0.
\end{align*}
$$

> Form now on we equal the following expressions $v=\gamma'(0)$
> $$
> [\gamma]f=vf=(f\circ \gamma)'(0)=\dfrac{\partial f}{\partial v}=\dfrac{\partial (f\circ \varphi^{-1})}{\partial v}|_{\varphi(0)}.
> $$

**Proposition** (change the basis of $T_pM$) Let $(U,\varphi,(x^1,\ldots,x^n))$ and $(V,\psi,(y^1,\ldots, y^n))$ be local coordinate system of $p\in M$. For arbitrary $f\in C^\infty(M)$, we have that
$$
\begin{align*}
\dfrac{\partial }{\partial x^i}f&=\dfrac{\partial (f\circ \varphi^{-1})}{\partial x^i}|_{\varphi(p)}\\[6pt]
&=\dfrac{\partial (f\circ \psi^{-1}\circ \psi\circ \varphi^{-1})}{\partial x^i}|_{\varphi(p)}\\[6pt]
&=\sum_\alpha\dfrac{\partial (f\circ \psi^{-1})}{\partial y^\alpha}|_{\psi(p)}\cdot \dfrac{\partial (\psi\circ \varphi^{-1})^\alpha}{\partial x^i}|_{\varphi(p)}\\[6pt]
&=\sum_\alpha \dfrac{\partial (\psi\circ \varphi^{-1})^\alpha}{\partial x^i}|_{\varphi(p)}\cdot \dfrac{\partial }{\partial y^\alpha} f.
\end{align*}
$$
Consequently, 
$$
\left(\dfrac{\partial }{\partial x^j}f\right)_{1\leq j\leq n}=\left(\dfrac{\partial (\psi\circ \varphi^{-1})^i}{\partial x^j}|_{\varphi(p)}\right)_{1\leq i,j\leq n}\cdot\left(\dfrac{\partial }{\partial y^i}f\right)_{1\leq i\leq n}.
$$